src/Std/Data/ExtDTreeMap/Basic.lean
@@ -724,7 +724,8 @@ def forM [TransCmp cmp] (f : (a : α) → β a → m PUnit) (t : ExtDTreeMap α 
   t.lift (fun m => m.forM f) (fun _ _ h => h.forM_eq (f := fun x => f x.1 x.2))
 
 @[inline, inherit_doc DTreeMap.forInNew]
-def forInNew [TransCmp cmp] (t : ExtDTreeMap α β cmp) (init : σ) (kcons : (a : α) → β a → (σ → m δ) → σ → m δ) (knil : σ → m δ) : m δ :=
+def forInNew {m : Type w → Type w₂} [TransCmp cmp] (t : ExtDTreeMap α β cmp) (init : σ)
+    (kcons : (a : α) → β a → (σ → m δ) → σ → m δ) (knil : σ → m δ) : m δ :=
   t.lift (fun m => m.forInNew init kcons knil) (fun _ _ h => h.forInNew_eq (kcons := fun x => kcons x.1 x.2))
 
 @[inline, inherit_doc DTreeMap.forIn]
@@ -753,6 +754,10 @@ define the `ForM` and `ForIn` instances for `ExtDTreeMap`.
 @[inline, inherit_doc ExtDTreeMap.forM]
 def forMUncurried [TransCmp cmp] (f : α × β → m PUnit) (t : ExtDTreeMap α β cmp) : m PUnit :=
   t.forM fun a b => f ⟨a, b⟩
+
+@[inline, inherit_doc ExtDTreeMap.forInNew]
+def forInNewUncurried {m : Type w → Type w₂} [TransCmp cmp] (t : ExtDTreeMap α β cmp) (init : σ) (kcons : α × β → (σ → m δ) → σ → m δ) (knil : σ → m δ) : m δ :=
+  t.forInNew init (fun a b => kcons ⟨a, b⟩) knil
 
 @[inline, inherit_doc ExtDTreeMap.forIn]
 def forInUncurried [TransCmp cmp] (f : α × β → δ → m (ForInStep δ)) (init : δ) (t : ExtDTreeMap α β cmp) : m δ :=
@@ -868,7 +873,7 @@ def mergeWith [TransCmp cmp] (mergeFn : α → β → β → β) (t₁ t₂ : Ex
 end Const
 
 @[inline, inherit_doc DTreeMap.insertMany]
-def insertMany [TransCmp cmp] {ρ} [ForIn Id ρ ((a : α) × β a)] (t : ExtDTreeMap α β cmp) (l : ρ) :
+def insertMany [TransCmp cmp] {ρ : Type w} [ForIn.{w, max u v, max u v, max u v} Id ρ ((a : α) × β a)] [ForInNew.{w, max u v, max u v, max u v} Id ρ ((a : α) × β a)] (t : ExtDTreeMap α β cmp) (l : ρ) :
     ExtDTreeMap α β cmp := Id.run do
   let mut acc : { a // ∀ P : _ → Prop, P t → (∀ t a b, P t → P (t.insert a b)) → P a } :=
     ⟨t, fun _ h _ => h⟩
@@ -877,7 +882,7 @@ def insertMany [TransCmp cmp] {ρ} [ForIn Id ρ ((a : α) × β a)] (t : ExtDTre
   return acc.1
 
 @[inline, inherit_doc DTreeMap.eraseMany]
-def eraseMany [TransCmp cmp] {ρ} [ForIn Id ρ α] (t : ExtDTreeMap α β cmp) (l : ρ) :
+def eraseMany [TransCmp cmp] {ρ : Type w} [ForIn.{w, u, max u v, max u v} Id ρ α] [ForInNew.{w, u, max u v, max u v} Id ρ α] (t : ExtDTreeMap α β cmp) (l : ρ) :
     ExtDTreeMap α β cmp := Id.run do
   let mut acc : { a // ∀ P : _ → Prop, P t → (∀ t a, P t → P (t.erase a)) → P a } :=
     ⟨t, fun _ h _ => h⟩
@@ -890,7 +895,7 @@ namespace Const
 variable {β : Type v}
 
 @[inline, inherit_doc ExtDTreeMap.insertMany]
-def insertMany [TransCmp cmp] {ρ} [ForIn Id ρ (α × β)] (t : ExtDTreeMap α β cmp) (l : ρ) :
+def insertMany [TransCmp cmp] {ρ : Type w} [ForIn.{w, max u v, max u v, max u v} Id ρ (α × β)] [ForInNew.{w, max u v, max u v, max u v} Id ρ (α × β)] (t : ExtDTreeMap α β cmp) (l : ρ) :
     ExtDTreeMap α β cmp := Id.run do
   let mut acc : { a // ∀ P : _ → Prop, P t → (∀ t a b, P t → P (t.insert a b)) → P a } :=
     ⟨t, fun _ h _ => h⟩
@@ -899,7 +904,7 @@ def insertMany [TransCmp cmp] {ρ} [ForIn Id ρ (α × β)] (t : ExtDTreeMap α 
   return acc.1
 
 @[inline, inherit_doc DTreeMap.Const.insertManyIfNewUnit]
-def insertManyIfNewUnit [TransCmp cmp] {ρ} [ForIn Id ρ α] (t : ExtDTreeMap α Unit cmp) (l : ρ) :
+def insertManyIfNewUnit [TransCmp cmp] {ρ : Type w} [ForIn.{w, u, u, u} Id ρ α] [ForInNew.{w, u, u, u} Id ρ α] (t : ExtDTreeMap α Unit cmp) (l : ρ) :
     ExtDTreeMap α Unit cmp := Id.run do
   let mut acc : { a // ∀ P : _ → Prop, P t → (∀ t a, P t → P (t.insertIfNew a ())) → P a } :=
     ⟨t, fun _ h _ => h⟩
